*** empty log message ***

doc-src/TutorialI/Datatype/Nested.thy
@@ -1,5 +1,5 @@
 (*<*)
-theory Nested = Main:;
+theory Nested = ABexpr:
 (*>*)
 
 text{*
@@ -12,18 +12,18 @@ where function symbols can be applied to a list of arguments:
 datatype ('a,'b)"term" = Var 'a | App 'b "('a,'b)term list";
 
 text{*\noindent
-Note that we need to quote \isa{term} on the left to avoid confusion with
+Note that we need to quote @{text"term"} on the left to avoid confusion with
 the command \isacommand{term}.
-Parameter \isa{'a} is the type of variables and \isa{'b} the type of
+Parameter @{typ"'a"} is the type of variables and @{typ"'b"} the type of
 function symbols.
 A mathematical term like $f(x,g(y))$ becomes @{term"App f [Var x, App g
-  [Var y]]"}, where \isa{f}, \isa{g}, \isa{x}, \isa{y} are
+  [Var y]]"}, where @{term"f"}, @{term"g"}, @{term"x"}, @{term"y"} are
 suitable values, e.g.\ numbers or strings.
 
-What complicates the definition of \isa{term} is the nested occurrence of
-\isa{term} inside \isa{list} on the right-hand side. In principle,
+What complicates the definition of @{text"term"} is the nested occurrence of
+@{text"term"} inside @{text"list"} on the right-hand side. In principle,
 nested recursion can be eliminated in favour of mutual recursion by unfolding
-the offending datatypes, here \isa{list}. The result for \isa{term}
+the offending datatypes, here @{text"list"}. The result for @{text"term"}
 would be something like
 \medskip
 
@@ -33,7 +33,7 @@ would be something like
 \noindent
 Although we do not recommend this unfolding to the user, it shows how to
 simulate nested recursion by mutual recursion.
-Now we return to the initial definition of \isa{term} using
+Now we return to the initial definition of @{text"term"} using
 nested recursion.
 
 Let us define a substitution function on terms. Because terms involve term
@@ -53,7 +53,7 @@ primrec
   "substs s (t # ts) = subst s t # substs s ts";
 
 text{*\noindent
-You should ignore the label \isa{subst\_App} for the moment.
+You should ignore the label @{thm[source]subst_App} for the moment.
 
 Similarly, when proving a statement about terms inductively, we need
 to prove a related statement about term lists simultaneously. For example,
@@ -66,39 +66,39 @@ lemma "subst  Var t  = (t ::('a,'b)term)  \\<and>
 by(induct_tac t and ts, simp_all);
 
 text{*\noindent
-Note that \isa{Var} is the identity substitution because by definition it
-leaves variables unchanged: @{term"subst Var (Var x) = Var x"}. Note also
+Note that @{term"Var"} is the identity substitution because by definition it
+leaves variables unchanged: @{prop"subst Var (Var x) = Var x"}. Note also
 that the type annotations are necessary because otherwise there is nothing in
 the goal to enforce that both halves of the goal talk about the same type
-parameters \isa{('a,'b)}. As a result, induction would fail
+parameters @{text"('a,'b)"}. As a result, induction would fail
 because the two halves of the goal would be unrelated.
 
 \begin{exercise}
 The fact that substitution distributes over composition can be expressed
 roughly as follows:
-\begin{ttbox}
-subst (f o g) t = subst f (subst g t)
-\end{ttbox}
+\begin{quote}
+@{text[display]"subst (f o g) t = subst f (subst g t)"}
+\end{quote}
 Correct this statement (you will find that it does not type-check),
-strengthen it, and prove it. (Note: \ttindexbold{o} is function composition;
-its definition is found in theorem \isa{o_def}).
+strengthen it, and prove it. (Note: \isaindexbold{o} is function composition;
+its definition is found in theorem @{thm[source]o_def}).
 \end{exercise}
 \begin{exercise}\label{ex:trev-trev}
-  Define a function \isa{trev} of type @{typ"('a,'b)term => ('a,'b)term"} that
-  recursively reverses the order of arguments of all function symbols in a
-  term. Prove that \isa{trev(trev t) = t}.
+  Define a function @{text"trev"} of type @{typ"('a,'b)term => ('a,'b)term"}
+that recursively reverses the order of arguments of all function symbols in a
+  term. Prove that @{prop"trev(trev t) = t"}.
 \end{exercise}
 
 The experienced functional programmer may feel that our above definition of
-\isa{subst} is unnecessarily complicated in that \isa{substs} is completely
-unnecessary. The @{term"App"}-case can be defined directly as
+@{term"subst"} is unnecessarily complicated in that @{term"substs"} is
+completely unnecessary. The @{term"App"}-case can be defined directly as
 \begin{quote}
 @{term[display]"subst s (App f ts) = App f (map (subst s) ts)"}
 \end{quote}
 where @{term"map"} is the standard list function such that
-\isa{map f [x1,...,xn] = [f x1,...,f xn]}. This is true, but Isabelle insists
-on the above fixed format. Fortunately, we can easily \emph{prove} that the
-suggested equation holds:
+@{text"map f [x1,...,xn] = [f x1,...,f xn]"}. This is true, but Isabelle
+insists on the above fixed format. Fortunately, we can easily \emph{prove}
+that the suggested equation holds:
 *}
 
 lemma [simp]: "subst s (App f ts) = App f (map (subst s) ts)"
@@ -115,15 +115,15 @@ text{*\noindent
 The advantage is that now we have replaced @{term"substs"} by
 @{term"map"}, we can profit from the large number of pre-proved lemmas
 about @{term"map"}.  Unfortunately inductive proofs about type
-\isa{term} are still awkward because they expect a conjunction. One
+@{text"term"} are still awkward because they expect a conjunction. One
 could derive a new induction principle as well (see
 \S\ref{sec:derive-ind}), but turns out to be simpler to define
 functions by \isacommand{recdef} instead of \isacommand{primrec}.
 The details are explained in \S\ref{sec:advanced-recdef} below.
 
 Of course, you may also combine mutual and nested recursion. For example,
-constructor \isa{Sum} in \S\ref{sec:datatype-mut-rec} could take a list of
-expressions as its argument: \isa{Sum "'a aexp list"}.
+constructor @{text"Sum"} in \S\ref{sec:datatype-mut-rec} could take a list of
+expressions as its argument: @{text"Sum"}~@{typ[quotes]"'a aexp list"}.
 *}
 (*<*)
 end
