doc-src/TutorialI/Datatype/Fundata.thy
@@ -3,11 +3,12 @@ theory Fundata = Main:
 (*>*)
 datatype ('a,'i)bigtree = Tip | Branch 'a "'i \\<Rightarrow> ('a,'i)bigtree"
 
-text{*\noindent Parameter \isa{'a} is the type of values stored in
-the \isa{Branch}es of the tree, whereas \isa{'i} is the index
-type over which the tree branches. If \isa{'i} is instantiated to
-\isa{bool}, the result is a binary tree; if it is instantiated to
-\isa{nat}, we have an infinitely branching tree because each node
+text{*\noindent
+Parameter @{typ"'a"} is the type of values stored in
+the @{term"Branch"}es of the tree, whereas @{typ"'i"} is the index
+type over which the tree branches. If @{typ"'i"} is instantiated to
+@{typ"bool"}, the result is a binary tree; if it is instantiated to
+@{typ"nat"}, we have an infinitely branching tree because each node
 has as many subtrees as there are natural numbers. How can we possibly
 write down such a tree? Using functional notation! For example, the term
 \begin{quote}
@@ -15,9 +16,9 @@ write down such a tree? Using functional notation! For example, the term
 \end{quote}
 of type @{typ"(nat,nat)bigtree"} is the tree whose
 root is labeled with 0 and whose $i$th subtree is labeled with $i$ and
-has merely \isa{Tip}s as further subtrees.
+has merely @{term"Tip"}s as further subtrees.
 
-Function \isa{map_bt} applies a function to all labels in a \isa{bigtree}:
+Function @{term"map_bt"} applies a function to all labels in a @{text"bigtree"}:
 *}
 
 consts map_bt :: "('a \\<Rightarrow> 'b) \\<Rightarrow> ('a,'i)bigtree \\<Rightarrow> ('b,'i)bigtree"
@@ -26,12 +27,12 @@ primrec
 "map_bt f (Branch a F) = Branch (f a) (\\<lambda>i. map_bt f (F i))"
 
 text{*\noindent This is a valid \isacommand{primrec} definition because the
-recursive calls of \isa{map_bt} involve only subtrees obtained from
-\isa{F}, i.e.\ the left-hand side. Thus termination is assured.  The
+recursive calls of @{term"map_bt"} involve only subtrees obtained from
+@{term"F"}, i.e.\ the left-hand side. Thus termination is assured.  The
 seasoned functional programmer might have written @{term"map_bt f o F"}
 instead of @{term"%i. map_bt f (F i)"}, but the former is not accepted by
 Isabelle because the termination proof is not as obvious since
-\isa{map_bt} is only partially applied.
+@{term"map_bt"} is only partially applied.
 
 The following lemma has a canonical proof  *}
 
