doc-src/TutorialI/Misc/AdvancedInd.thy
@@ -21,7 +21,7 @@ lemma "xs \\<noteq> [] \\<Longrightarrow> hd(rev xs) = last xs";
 apply(induct_tac xs);
 
 txt{*\noindent
-(where \isa{hd} and \isa{last} return the first and last element of a
+(where @{term"hd"} and @{term"last"} return the first and last element of a
 non-empty list)
 produces the warning
 \begin{quote}\tt
@@ -35,16 +35,16 @@ which, after simplification, becomes
 \begin{isabelle}
 \ 1.\ xs\ {\isasymnoteq}\ []\ {\isasymLongrightarrow}\ hd\ []\ =\ last\ []
 \end{isabelle}
-We cannot prove this equality because we do not know what \isa{hd} and
-\isa{last} return when applied to \isa{[]}.
+We cannot prove this equality because we do not know what @{term"hd"} and
+@{term"last"} return when applied to @{term"[]"}.
 
 The point is that we have violated the above warning. Because the induction
-formula is only the conclusion, the occurrence of \isa{xs} in the premises is
+formula is only the conclusion, the occurrence of @{term"xs"} in the premises is
 not modified by induction. Thus the case that should have been trivial
 becomes unprovable. Fortunately, the solution is easy:
 \begin{quote}
 \emph{Pull all occurrences of the induction variable into the conclusion
-using \isa{\isasymlongrightarrow}.}
+using @{text"\<longrightarrow>"}.}
 \end{quote}
 This means we should prove
 *};
@@ -59,12 +59,13 @@ This time, induction leaves us with the following base case
 \begin{isabelle}
 \ 1.\ []\ {\isasymnoteq}\ []\ {\isasymlongrightarrow}\ hd\ (rev\ [])\ =\ last\ []
 \end{isabelle}
-which is trivial, and \isa{auto} finishes the whole proof.
+which is trivial, and @{text"auto"} finishes the whole proof.
 
-If \isa{hd\_rev} is meant to be a simplification rule, you are done. But if you
-really need the \isa{\isasymLongrightarrow}-version of \isa{hd\_rev}, for
-example because you want to apply it as an introduction rule, you need to
-derive it separately, by combining it with modus ponens:
+If @{thm[source]hd_rev} is meant to be a simplification rule, you are
+done. But if you really need the @{text"\<Longrightarrow>"}-version of
+@{thm[source]hd_rev}, for example because you want to apply it as an
+introduction rule, you need to derive it separately, by combining it with
+modus ponens:
 *};
 
 lemmas hd_revI = hd_rev[THEN mp];
@@ -78,7 +79,7 @@ induction variable, you should turn the conclusion $C$ into
 (see the remark?? in \S\ref{??}).
 Additionally, you may also have to universally quantify some other variables,
 which can yield a fairly complex conclusion.
-Here is a simple example (which is proved by \isa{blast}):
+Here is a simple example (which is proved by @{text"blast"}):
 *};
 
 lemma simple: "\\<forall>y. A y \\<longrightarrow> B y \<longrightarrow> B y & A y";
@@ -86,14 +87,14 @@ lemma simple: "\\<forall>y. A y \\<longrightarrow> B y \<longrightarrow> B y & A
 
 text{*\noindent
 You can get the desired lemma by explicit
-application of modus ponens and \isa{spec}:
+application of modus ponens and @{thm[source]spec}:
 *};
 
 lemmas myrule = simple[THEN spec, THEN mp, THEN mp];
 
 text{*\noindent
-or the wholesale stripping of \isa{\isasymforall} and
-\isa{\isasymlongrightarrow} in the conclusion via \isa{rulify} 
+or the wholesale stripping of @{text"\<forall>"} and
+@{text"\<longrightarrow>"} in the conclusion via @{text"rulify"} 
 *};
 
 lemmas myrule = simple[rulify];
@@ -130,10 +131,10 @@ recursive function in sight either that could furnish a more appropriate
 induction schema. In such cases some existing standard induction schema can
 be helpful. We show how to apply such induction schemas by an example.
 
-Structural induction on \isa{nat} is
+Structural induction on @{typ"nat"} is
 usually known as ``mathematical induction''. There is also ``complete
 induction'', where you must prove $P(n)$ under the assumption that $P(m)$
-holds for all $m<n$. In Isabelle, this is the theorem \isa{less\_induct}:
+holds for all $m<n$. In Isabelle, this is the theorem @{thm[source]less_induct}:
 \begin{quote}
 @{thm[display]"less_induct"[no_vars]}
 \end{quote}
@@ -148,7 +149,7 @@ From the above axiom\footnote{In general, the use of axioms is strongly
 discouraged, because of the danger of inconsistencies. The above axiom does
 not introduce an inconsistency because, for example, the identity function
 satisfies it.}
-for \isa{f} it follows that @{term"n <= f n"}, which can
+for @{term"f"} it follows that @{prop"n <= f n"}, which can
 be proved by induction on @{term"f n"}. Following the recipy outlined
 above, we have to phrase the proposition as follows to allow induction:
 *};
@@ -156,7 +157,7 @@ above, we have to phrase the proposition as follows to allow induction:
 lemma f_incr_lem: "\\<forall>i. k = f i \\<longrightarrow> i \\<le> f i";
 
 txt{*\noindent
-To perform induction on \isa{k} using \isa{less\_induct}, we use the same
+To perform induction on @{term"k"} using @{thm[source]less_induct}, we use the same
 general induction method as for recursion induction (see
 \S\ref{sec:recdef-induction}):
 *};
@@ -173,9 +174,9 @@ which leaves us with the following proof state:
 \ 1.\ {\isasymAnd}\mbox{n}.\ {\isasymforall}\mbox{m}.\ \mbox{m}\ <\ \mbox{n}\ {\isasymlongrightarrow}\ ({\isasymforall}\mbox{i}.\ \mbox{m}\ =\ f\ \mbox{i}\ {\isasymlongrightarrow}\ \mbox{i}\ {\isasymle}\ f\ \mbox{i})\isanewline
 \ \ \ \ \ \ \ {\isasymLongrightarrow}\ {\isasymforall}\mbox{i}.\ \mbox{n}\ =\ f\ \mbox{i}\ {\isasymlongrightarrow}\ \mbox{i}\ {\isasymle}\ f\ \mbox{i}
 \end{isabelle}
-After stripping the \isa{\isasymforall i}, the proof continues with a case
-distinction on \isa{i}. The case \isa{i = 0} is trivial and we focus on the
-other case:
+After stripping the @{text"\<forall>i"}, the proof continues with a case
+distinction on @{term"i"}. The case @{prop"i = 0"} is trivial and we focus on
+the other case:
 \begin{isabelle}
 \ 1.\ {\isasymAnd}\mbox{n}\ \mbox{i}\ \mbox{nat}.\isanewline
 \ \ \ \ \ \ \ {\isasymlbrakk}{\isasymforall}\mbox{m}.\ \mbox{m}\ <\ \mbox{n}\ {\isasymlongrightarrow}\ ({\isasymforall}\mbox{i}.\ \mbox{m}\ =\ f\ \mbox{i}\ {\isasymlongrightarrow}\ \mbox{i}\ {\isasymle}\ f\ \mbox{i});\ \mbox{i}\ =\ Suc\ \mbox{nat}{\isasymrbrakk}\isanewline
@@ -187,16 +188,16 @@ by(blast intro!: f_ax Suc_leI intro:le_less_trans);
 
 text{*\noindent
 It is not surprising if you find the last step puzzling.
-The proof goes like this (writing \isa{j} instead of \isa{nat}).
-Since @{term"i = Suc j"} it suffices to show
-@{term"j < f(Suc j)"} (by \isa{Suc\_leI}: @{thm"Suc_leI"[no_vars]}). This is
-proved as follows. From \isa{f\_ax} we have @{term"f (f j) < f (Suc j)"}
-(1) which implies @{term"f j <= f (f j)"} (by the induction hypothesis).
-Using (1) once more we obtain @{term"f j < f(Suc j)"} (2) by transitivity
-(\isa{le_less_trans}: @{thm"le_less_trans"[no_vars]}).
-Using the induction hypothesis once more we obtain @{term"j <= f j"}
-which, together with (2) yields @{term"j < f (Suc j)"} (again by
-\isa{le_less_trans}).
+The proof goes like this (writing @{term"j"} instead of @{typ"nat"}).
+Since @{prop"i = Suc j"} it suffices to show
+@{prop"j < f(Suc j)"} (by @{thm[source]Suc_leI}: @{thm"Suc_leI"[no_vars]}). This is
+proved as follows. From @{thm[source]f_ax} we have @{prop"f (f j) < f (Suc j)"}
+(1) which implies @{prop"f j <= f (f j)"} (by the induction hypothesis).
+Using (1) once more we obtain @{prop"f j < f(Suc j)"} (2) by transitivity
+(@{thm[source]le_less_trans}: @{thm"le_less_trans"[no_vars]}).
+Using the induction hypothesis once more we obtain @{prop"j <= f j"}
+which, together with (2) yields @{prop"j < f (Suc j)"} (again by
+@{thm[source]le_less_trans}).
 
 This last step shows both the power and the danger of automatic proofs: they
 will usually not tell you how the proof goes, because it can be very hard to
@@ -204,14 +205,14 @@ translate the internal proof into a human-readable format. Therefore
 \S\ref{sec:part2?} introduces a language for writing readable yet concise
 proofs.
 
-We can now derive the desired @{term"i <= f i"} from \isa{f\_incr}:
+We can now derive the desired @{prop"i <= f i"} from @{text"f_incr"}:
 *};
 
 lemmas f_incr = f_incr_lem[rulify, OF refl];
 
 text{*\noindent
-The final \isa{refl} gets rid of the premise \isa{?k = f ?i}. Again, we could
-have included this derivation in the original statement of the lemma:
+The final @{thm[source]refl} gets rid of the premise @{text"?k = f ?i"}. Again,
+we could have included this derivation in the original statement of the lemma:
 *};
 
 lemma f_incr[rulify, OF refl]: "\\<forall>i. k = f i \\<longrightarrow> i \\<le> f i";
@@ -219,22 +220,23 @@ lemma f_incr[rulify, OF refl]: "\\<forall>i. k = f i \\<longrightarrow> i \\<le>
 
 text{*
 \begin{exercise}
-From the above axiom and lemma for \isa{f} show that \isa{f} is the identity.
+From the above axiom and lemma for @{term"f"} show that @{term"f"} is the
+identity.
 \end{exercise}
 
-In general, \isa{induct\_tac} can be applied with any rule \isa{r}
-whose conclusion is of the form \isa{?P ?x1 \dots ?xn}, in which case the
+In general, @{text"induct_tac"} can be applied with any rule $r$
+whose conclusion is of the form ${?}P~?x@1 \dots ?x@n$, in which case the
 format is
-\begin{ttbox}
-apply(induct_tac y1 ... yn rule: r)
-\end{ttbox}\index{*induct_tac}%
-where \isa{y1}, \dots, \isa{yn} are variables in the first subgoal.
-In fact, \isa{induct\_tac} even allows the conclusion of
-\isa{r} to be an (iterated) conjunction of formulae of the above form, in
+\begin{quote}
+\isacommand{apply}@{text"(induct_tac"} $y@1 \dots y@n$ @{text"rule:"} $r$@{text")"}
+\end{quote}\index{*induct_tac}%
+where $y@1, \dots, y@n$ are variables in the first subgoal.
+In fact, @{text"induct_tac"} even allows the conclusion of
+$r$ to be an (iterated) conjunction of formulae of the above form, in
 which case the application is
-\begin{ttbox}
-apply(induct_tac y1 ... yn and ... and z1 ... zm rule: r)
-\end{ttbox}
+\begin{quote}
+\isacommand{apply}@{text"(induct_tac"} $y@1 \dots y@n$ @{text"and"} \dots\ @{text"and"} $z@1 \dots z@m$ @{text"rule:"} $r$@{text")"}
+\end{quote}
 *};
 
 subsection{*Derivation of new induction schemas*};
@@ -242,18 +244,18 @@ subsection{*Derivation of new induction schemas*};
 text{*\label{sec:derive-ind}
 Induction schemas are ordinary theorems and you can derive new ones
 whenever you wish.  This section shows you how to, using the example
-of \isa{less\_induct}. Assume we only have structural induction
+of @{thm[source]less_induct}. Assume we only have structural induction
 available for @{typ"nat"} and want to derive complete induction. This
 requires us to generalize the statement first:
 *};
 
-lemma induct_lem: "(\\<And>n::nat. \\<forall>m<n. P m \\<Longrightarrow> P n) ==> \\<forall>m<n. P m";
+lemma induct_lem: "(\\<And>n::nat. \\<forall>m<n. P m \\<Longrightarrow> P n) \\<Longrightarrow> \\<forall>m<n. P m";
 apply(induct_tac n);
 
 txt{*\noindent
-The base case is trivially true. For the induction step (@{term"m <
-Suc n"}) we distinguish two cases: @{term"m < n"} is true by induction
-hypothesis and @{term"m = n"} follow from the assumption again using
+The base case is trivially true. For the induction step (@{prop"m <
+Suc n"}) we distinguish two cases: @{prop"m < n"} is true by induction
+hypothesis and @{prop"m = n"} follow from the assumption again using
 the induction hypothesis:
 *};
 
@@ -264,31 +266,31 @@ sorry;
 ML"reset quick_and_dirty"
 
 text{*\noindent
-The elimination rule \isa{less_SucE} expresses the case distinction:
+The elimination rule @{thm[source]less_SucE} expresses the case distinction:
 \begin{quote}
 @{thm[display]"less_SucE"[no_vars]}
 \end{quote}
 
 Now it is straightforward to derive the original version of
-\isa{less\_induct} by manipulting the conclusion of the above lemma:
-instantiate \isa{n} by @{term"Suc n"} and \isa{m} by \isa{n} and
-remove the trivial condition @{term"n < Sc n"}. Fortunately, this
+@{thm[source]less_induct} by manipulting the conclusion of the above lemma:
+instantiate @{term"n"} by @{term"Suc n"} and @{term"m"} by @{term"n"} and
+remove the trivial condition @{prop"n < Sc n"}. Fortunately, this
 happens automatically when we add the lemma as a new premise to the
 desired goal:
 *};
 
-theorem less_induct: "(\\<And>n::nat. \\<forall>m<n. P m \\<Longrightarrow> P n) ==> P n";
+theorem less_induct: "(\\<And>n::nat. \\<forall>m<n. P m \\<Longrightarrow> P n) \\<Longrightarrow> P n";
 by(insert induct_lem, blast);
 
 text{*\noindent
 Finally we should mention that HOL already provides the mother of all
-inductions, \emph{wellfounded induction} (\isa{wf\_induct}):
+inductions, \emph{wellfounded induction} (@{thm[source]wf_induct}):
 \begin{quote}
 @{thm[display]"wf_induct"[no_vars]}
 \end{quote}
-where @{term"wf r"} means that the relation \isa{r} is wellfounded.
-For example \isa{less\_induct} is the special case where \isa{r} is \isa{<} on @{typ"nat"}.
-For details see the library.
+where @{term"wf r"} means that the relation @{term"r"} is wellfounded.
+For example @{thm[source]less_induct} is the special case where @{term"r"} is
+@{text"<"} on @{typ"nat"}. For details see the library.
 *};
 
 (*<*)
