doc-src/TutorialI/Misc/case_splits.thy
@@ -3,8 +3,8 @@ theory case_splits = Main:;
 (*>*)
 
 text{*
-Goals containing \isaindex{if}-expressions are usually proved by case
-distinction on the condition of the \isa{if}. For example the goal
+Goals containing @{text"if"}-expressions are usually proved by case
+distinction on the condition of the @{text"if"}. For example the goal
 *}
 
 lemma "\\<forall>xs. if xs = [] then rev xs = [] else rev xs \\<noteq> []";
@@ -12,7 +12,7 @@ lemma "\\<forall>xs. if xs = [] then rev xs = [] else rev xs \\<noteq> []";
 txt{*\noindent
 can be split into
 \begin{isabelle}
-~1.~{\isasymforall}xs.~(xs~=~[]~{\isasymlongrightarrow}~rev~xs~=~[])~{\isasymand}~(xs~{\isasymnoteq}~[]~{\isasymlongrightarrow}~rev~xs~{\isasymnoteq}~[])%
+~1.~{\isasymforall}xs.~(xs~=~[]~{\isasymlongrightarrow}~rev~xs~=~[])~{\isasymand}~(xs~{\isasymnoteq}~[]~{\isasymlongrightarrow}~rev~xs~{\isasymnoteq}~[])
 \end{isabelle}
 by a degenerate form of simplification
 *}
@@ -21,14 +21,14 @@ apply(simp only: split: split_if);
 (*<*)oops;(*>*)
 
 text{*\noindent
-where no simplification rules are included (\isa{only:} is followed by the
+where no simplification rules are included (@{text"only:"} is followed by the
 empty list of theorems) but the rule \isaindexbold{split_if} for
-splitting \isa{if}s is added (via the modifier \isa{split:}). Because
-case-splitting on \isa{if}s is almost always the right proof strategy, the
-simplifier performs it automatically. Try \isacommand{apply}\isa{(simp)}
+splitting @{text"if"}s is added (via the modifier @{text"split:"}). Because
+case-splitting on @{text"if"}s is almost always the right proof strategy, the
+simplifier performs it automatically. Try \isacommand{apply}@{text"(simp)"}
 on the initial goal above.
 
-This splitting idea generalizes from \isa{if} to \isaindex{case}:
+This splitting idea generalizes from @{text"if"} to \isaindex{case}:
 *}
 
 lemma "(case xs of [] \\<Rightarrow> zs | y#ys \\<Rightarrow> y#(ys@zs)) = xs@zs";
@@ -36,7 +36,7 @@ txt{*\noindent
 becomes
 \begin{isabelle}
 ~1.~(xs~=~[]~{\isasymlongrightarrow}~zs~=~xs~@~zs)~{\isasymand}\isanewline
-~~~~({\isasymforall}a~list.~xs~=~a~\#~list~{\isasymlongrightarrow}~a~\#~list~@~zs~=~xs~@~zs)%
+~~~~({\isasymforall}a~list.~xs~=~a~\#~list~{\isasymlongrightarrow}~a~\#~list~@~zs~=~xs~@~zs)
 \end{isabelle}
 by typing
 *}
@@ -45,9 +45,9 @@ apply(simp only: split: list.split);
 (*<*)oops;(*>*)
 
 text{*\noindent
-In contrast to \isa{if}-expressions, the simplifier does not split
-\isa{case}-expressions by default because this can lead to nontermination
-in case of recursive datatypes. Again, if the \isa{only:} modifier is
+In contrast to @{text"if"}-expressions, the simplifier does not split
+@{text"case"}-expressions by default because this can lead to nontermination
+in case of recursive datatypes. Again, if the @{text"only:"} modifier is
 dropped, the above goal is solved,
 *}
 (*<*)
@@ -56,17 +56,17 @@ lemma "(case xs of [] \\<Rightarrow> zs | y#ys \\<Rightarrow> y#(ys@zs)) = xs@zs
 by(simp split: list.split);
 
 text{*\noindent%
-which \isacommand{apply}\isa{(simp)} alone will not do.
+which \isacommand{apply}@{text"(simp)"} alone will not do.
 
 In general, every datatype $t$ comes with a theorem
-\isa{$t$.split} which can be declared to be a \bfindex{split rule} either
-locally as above, or by giving it the \isa{split} attribute globally:
+$t$@{text".split"} which can be declared to be a \bfindex{split rule} either
+locally as above, or by giving it the @{text"split"} attribute globally:
 *}
 
 lemmas [split] = list.split;
 
 text{*\noindent
-The \isa{split} attribute can be removed with the \isa{del} modifier,
+The @{text"split"} attribute can be removed with the @{text"del"} modifier,
 either locally
 *}
 (*<*)
@@ -83,8 +83,9 @@ lemmas [split del] = list.split;
 
 text{*
 The above split rules intentionally only affect the conclusion of a
-subgoal.  If you want to split an \isa{if} or \isa{case}-expression in
-the assumptions, you have to apply \isa{split\_if\_asm} or $t$\isa{.split_asm}:
+subgoal.  If you want to split an @{text"if"} or @{text"case"}-expression in
+the assumptions, you have to apply @{thm[source]split_if_asm} or
+$t$@{text".split_asm"}:
 *}
 
 lemma "if xs = [] then ys ~= [] else ys = [] ==> xs @ ys ~= []"
@@ -92,13 +93,14 @@ apply(simp only: split: split_if_asm);
 
 txt{*\noindent
 In contrast to splitting the conclusion, this actually creates two
-separate subgoals (which are solved by \isa{simp\_all}):
+separate subgoals (which are solved by @{text"simp_all"}):
 \begin{isabelle}
 \ \isadigit{1}{\isachardot}\ {\isasymlbrakk}\mbox{xs}\ {\isacharequal}\ {\isacharbrackleft}{\isacharbrackright}{\isacharsemicolon}\ \mbox{ys}\ {\isasymnoteq}\ {\isacharbrackleft}{\isacharbrackright}{\isasymrbrakk}\ {\isasymLongrightarrow}\ {\isacharbrackleft}{\isacharbrackright}\ {\isacharat}\ \mbox{ys}\ {\isasymnoteq}\ {\isacharbrackleft}{\isacharbrackright}\isanewline
 \ \isadigit{2}{\isachardot}\ {\isasymlbrakk}\mbox{xs}\ {\isasymnoteq}\ {\isacharbrackleft}{\isacharbrackright}{\isacharsemicolon}\ \mbox{ys}\ {\isacharequal}\ {\isacharbrackleft}{\isacharbrackright}{\isasymrbrakk}\ {\isasymLongrightarrow}\ \mbox{xs}\ {\isacharat}\ {\isacharbrackleft}{\isacharbrackright}\ {\isasymnoteq}\ {\isacharbrackleft}{\isacharbrackright}
 \end{isabelle}
 If you need to split both in the assumptions and the conclusion,
-use $t$\isa{.splits} which subsumes $t$\isa{.split} and $t$\isa{.split_asm}.
+use $t$@{text".splits"} which subsumes $t$@{text".split"} and
+$t$@{text".split_asm"}. Analogously, there is @{thm[source]if_splits}.
 *}
 
 (*<*)
