doc-src/TutorialI/Misc/cond_rewr.thy
@@ -23,10 +23,10 @@ by(simp);
 (*>*)
 text{*\noindent
 is proved by plain simplification:
-the conditional equation \isa{hd_Cons_tl} above
-can simplify \isa{hd(rev~xs)~\#~tl(rev~xs)} to \isa{rev xs}
-because the corresponding precondition \isa{rev xs \isasymnoteq\ []}
-simplifies to \isa{xs \isasymnoteq\ []}, which is exactly the local
+the conditional equation @{thm[source]hd_Cons_tl} above
+can simplify @{term"hd(rev xs) # tl(rev xs)"} to @{term"rev xs"}
+because the corresponding precondition @{term"rev xs ~= []"}
+simplifies to @{term"xs ~= []"}, which is exactly the local
 assumption of the subgoal.
 *}
 (*<*)
